proof/refine/AARCH64/Arch_R.thy
@@ -315,7 +315,8 @@ lemma performASIDControlInvocation_corres:
          rule pspace_no_overlap_detype[OF caps_of_state_valid])
         apply (simp add:invs_psp_aligned invs_valid_objs is_aligned_neg_mask_eq)+
    apply (clarsimp simp: detype_def clear_um_def detype_ext_def valid_sched_def valid_etcbs_def
-            st_tcb_at_kh_def obj_at_kh_def st_tcb_at_def obj_at_def is_etcb_at_def)
+                         st_tcb_at_kh_def obj_at_kh_def st_tcb_at_def obj_at_def is_etcb_at_def
+                         wrap_ext_det_ext_ext_def)
   apply (simp add: detype_def clear_um_def)
   apply (drule_tac x = "cte_map (aa,ba)" in pspace_relation_cte_wp_atI[OF state_relation_pspace_relation])
     apply (simp add:invs_valid_objs)+
@@ -328,9 +329,9 @@ lemma performASIDControlInvocation_corres:
   apply clarsimp
   apply (frule empty_descendants_range_in')
   apply (intro conjI,
-    simp_all add: is_simple_cap'_def isCap_simps descendants_range'_def2
-                  null_filter_descendants_of'[OF null_filter_simp']
-                  capAligned_def asid_low_bits_def)
+         simp_all add: is_simple_cap'_def isCap_simps descendants_range'_def2
+                       null_filter_descendants_of'[OF null_filter_simp']
+                       capAligned_def asid_low_bits_def)
       apply (erule descendants_range_caps_no_overlapI')
        apply (fastforce simp:cte_wp_at_ctes_of is_aligned_neg_mask_eq)
       apply (simp add:empty_descendants_range_in')
